mm0-lean/x86/matching.lean
@@ -45,6 +45,10 @@ def place.stable (k k' : config) : place → Prop
 theorem place.stable.refl (k p) : place.stable k k p :=
 by cases p; exact rfl
 
+theorem place.stable.trans {k₁ k₂ k₃ p}
+  (h₁ : place.stable k₁ k₂ p) (h₂ : place.stable k₂ k₃ p) : place.stable k₁ k₃ p :=
+by cases p; exact eq.trans h₁ h₂
+
 theorem mem.read1.stable {k k' a} (s : place.stable k k' (place.mem a))
   {p b} : mem.read1 p k.mem a b → mem.read1 p k'.mem a b :=
 @@eq.subst (λ o : roption (byte × perm),
@@ -62,7 +66,7 @@ end
 
 def stability (k k' : config) : set place := {p | place.stable k k' p}
 
-def split (H h₁ h₂ : set place) : Prop :=
+def split {α} (H h₁ h₂ : set α) : Prop :=
 H = h₁ ∪ h₂ ∧ disjoint h₁ h₂
 
 def sProp := config → Prop
@@ -83,10 +87,16 @@ def mProp := config → config → Prop
 def mProp.exterior (P : mProp) : set place :=
 {p | ∀ k k', P k k' → place.stable k k' p}
 
+def mProp.dom (P : mProp) : set place := -P.exterior
+
 def stable_at (D : set place) : mProp := λ k k', D ⊆ stability k k'
 
-theorem stable_at.zero {D k} : stable_at D k k :=
+theorem stable_at.refl {D k} : stable_at D k k :=
 λ x _, place.stable.refl _ _
+
+theorem stable_at.trans {D k₁ k₂ k₃}
+  (h₁ : stable_at D k₁ k₂) (h₂ : stable_at D k₂ k₃) : stable_at D k₁ k₃ :=
+λ x h, place.stable.trans (h₁ h) (h₂ h)
 
 def mProp.initial (Q : mProp) (P : sProp) : mProp := λ k k', Q k k' ∧ P k
 def mProp.final (Q : mProp) (P : sProp) : mProp := λ k k', Q k k' ∧ P k'
@@ -97,27 +107,20 @@ def mProp.apply (Q : mProp) (P : sProp) : sProp :=
 def mProp.id : mProp := eq
 
 def mProp.comp (P Q : mProp) : mProp :=
-λ k k₂, ∃ k₁, P k k₁ ∧ Q k₁ k₂
+λ k₁ k₃, ∃ k₂, P k₁ k₂ ∧ Q k₂ k₃
+
+def mProp.imp (P Q : mProp) : mProp :=
+λ k₂ k₃, ∀ k₁, P k₁ k₂ → Q k₁ k₃
 
 def slift (p : Prop) : sProp := λ _, p
 def mlift (p : Prop) : mProp := λ _ _, p
 
-instance has_le.mProp : has_le mProp := ⟨λ P Q, ∀ {{k k'}}, P k k' → Q k k'⟩
-instance has_le.sProp : has_le sProp := ⟨λ P Q, ∀ {{k}}, P k → Q k⟩
+open lattice
+instance lattice.complete_lattice.sProp : complete_lattice sProp :=
+pi.complete_lattice
 
-def sProp.and (P Q : sProp) : sProp := λ k, P k ∧ Q k
-def mProp.and (P Q : mProp) : mProp := λ k k', P k k' ∧ Q k k'
-def sProp.or (P Q : sProp) : sProp := λ k, P k ∨ Q k
-def mProp.or (P Q : mProp) : mProp := λ k k', P k k' ∨ Q k k'
-instance lattice.has_inf.sProp : lattice.has_inf sProp := ⟨sProp.and⟩
-instance lattice.has_inf.mProp : lattice.has_inf mProp := ⟨mProp.and⟩
-instance lattice.has_sup.sProp : lattice.has_sup sProp := ⟨sProp.or⟩
-instance lattice.has_sup.mProp : lattice.has_sup mProp := ⟨mProp.or⟩
-
-instance lattice.has_top.sProp : lattice.has_top sProp := ⟨λ _, true⟩
-instance lattice.has_top.mProp : lattice.has_top mProp := ⟨λ _ _, true⟩
-instance lattice.has_bot.sProp : lattice.has_bot sProp := ⟨λ _, false⟩
-instance lattice.has_bot.mProp : lattice.has_bot mProp := ⟨λ _ _, false⟩
+instance lattice.complete_lattice.mProp : complete_lattice mProp :=
+pi.complete_lattice
 
 def sProp.with (p : sProp) (q : Prop) : sProp := p ⊓ slift q
 def mProp.with (p : mProp) (q : Prop) : mProp := p ⊓ mlift q
@@ -164,17 +167,17 @@ def sProp.mem_block (p : perm) (a : qword) (v : list byte) : sProp :=
 
 def block.read : block → list byte → sProp
 | (block.reg r sz) v :=
-  (sProp.reserve (block.reg r sz).places).and $ λ k,
+  (sProp.reserve (block.reg r sz).places) ⊓ λ k,
     read_full_imm sz (k.regs r) v
 | (block.mem a sz) v :=
-  (sProp.reserve (block.mem a sz).places).and $ λ k,
+  (sProp.reserve (block.mem a sz).places) ⊓ λ k,
     k.mem.read a v ∧ v.length = sz.to_nat
 | (block.const l) v := slift $ v = l
 
 def block.writable : block → sProp
 | (block.reg r sz) := sProp.reserve (block.reg r sz).places
 | (block.mem a sz) :=
-  (sProp.reserve (block.mem a sz).places).and $ λ k,
+  (sProp.reserve (block.mem a sz).places) ⊓ λ k,
     ∃ v, k.mem.read' perm.W a v ∧ v.length = sz.to_nat
 | (block.const _) := slift false
 
@@ -199,15 +202,6 @@ theorem block.read.stable {l v k k'}
   (h₁ : block.read l v k) (ss : places l ⊆ stability k k') :
   block.read l v k' := sorry
 
-def locals_ctx := alist (λ _ : ℕ, block)
-
-def locals_ctx.get (Γ : locals_ctx) (n : ℕ) : option block := Γ.lookup n
-
-def labels_ctx := qword × list qword
-
-def labels_ctx.cons (q : qword) (L : labels_ctx) : labels_ctx :=
-⟨L.1, q :: L.2⟩
-
 inductive hoare_p (Q : kcfg → Prop) : kcfg → Prop
 | zero {{k}} : Q k → hoare_p k
 | step {{k}} : (∃ k', kcfg.step k k') →
@@ -219,73 +213,96 @@ def hoare (P : kcfg → Prop) (Q : kcfg → kcfg → Prop) :=
 ∀ {{k}}, P k → hoare_p (Q k) k
 
 def mHoareIO (P : sProp) (Q : list byte → list byte → mProp) :=
-∀ {{i o}}, hoare (λ k, P k.k ∧ k.input = i ∧ k.output = o)
-  (λ k k', ∃ i' o', i = i' ++ k.input ∧ o = k.output ++ o' ∧
+hoare (λ k, P k.k)
+  (λ k k', ∃ i' o', k.input = i' ++ k'.input ∧ k'.output = k.output ++ o' ∧
     (Q i' o') k.k k'.k)
 
 def noIO (Q : mProp) (i o : list byte) : mProp := Q.with (i = [] ∧ o = [])
 def mHoare (P : sProp) (Q : mProp) := mHoareIO P (noIO Q)
 
+def locals_ctx := alist (λ _ : ℕ, block)
+
+def locals_ctx.get (Γ : locals_ctx) (n : ℕ) : option block := Γ.lookup n
+
+def labels_ctx := qword × list qword
+
+def labels_ctx.cons (q : qword) (L : labels_ctx) : labels_ctx :=
+⟨L.1, q :: L.2⟩
+
+structure asm_ctx :=
+(L : list qword)
+(Γ : alist (λ _ : ℕ, block))
+(exit : qword)
+(die : ∃ l, mHoare (sProp.sn place.rip exit ⊓
+  sProp.mem_block (perm.R + perm.X) exit l) ⊥)
+
+def asm_ctx.read (A : asm_ctx) (n : ℕ) : option block := A.Γ.lookup n
+
+def asm_ctx.push_local (A : asm_ctx) (i : ℕ) (b : block) : asm_ctx :=
+⟨A.1, A.2.insert i b, A.3, A.4⟩
+
+def asm_ctx.push_label (A : asm_ctx) (q : qword) : asm_ctx :=
+⟨q :: A.1, A.2, A.3, A.4⟩
+
 inductive exit_kind
 | straight
 | label (n : ℕ)
 
-def exit_kind.result (L : labels_ctx) (pos : qword) : exit_kind → mProp
-| exit_kind.straight := mProp.write place.rip pos
-| (exit_kind.label n) := mProp.ex $ λ h, mProp.write place.rip (L.2.nth_le n h)
+def exit_kind.result (A : asm_ctx) (pos : qword) : exit_kind → sProp
+| exit_kind.straight := sProp.sn place.rip pos
+| (exit_kind.label n) := sProp.ex $ λ h, sProp.sn place.rip (A.1.nth_le n h)
 
 def stmt : Type :=
-labels_ctx → locals_ctx → set place →
+asm_ctx → set place →
 ∀ rip : qword, list byte → Prop
 
-def stmt.hoareIO (L Γ) (P : sProp) (C : stmt)
+def stmt.hoareIO (A) (P : sProp) (C : stmt)
   (Q : exit_kind → list byte → list byte → mProp) : Prop :=
-∀ D rip l, C L Γ D rip l →
+∀ D rip l, C A D rip l →
   mHoareIO
     (P ⊓ sProp.sn place.rip rip ⊓
       sProp.mem_block (perm.R + perm.X) rip l)
     (λ i o, stable_at D ⊓
-      (mProp.write place.rip L.1 ⊔
-       mProp.ex (λ e, Q e i o ⊓ e.result L (rip + l.length))))
+      mProp.ex (λ e, (Q e i o).final (e.result A (rip + l.length))))
 
-def stmt.hoare (L Γ) (P : sProp) (C : stmt) (Q : exit_kind → mProp) : Prop :=
-stmt.hoareIO L Γ P C (λ e i o, noIO (Q e) i o)
+def stmt.hoare (A) (P : sProp) (C : stmt) (Q : exit_kind → mProp) : Prop :=
+stmt.hoareIO A P C (λ e i o, noIO (Q e) i o)
 
 def hstmt (P : sProp) (Q : mProp) : stmt :=
-λ L Γ D rip v,
+λ A D rip v,
   mHoare (sProp.sn place.rip rip ⊓ sProp.mem_block (perm.R + perm.X) rip v)
-    (Q ⊓ stable_at D ⊓ mProp.write place.rip (rip + v.length))
+    ((Q ⊓ stable_at D).final (sProp.sn place.rip (rip + v.length)))
 
-instance has_le.stmt : has_le stmt :=
-⟨λ s t, ∀ {{L Γ D rip v}}, s L Γ D rip v → t L Γ D rip v⟩
+instance complete_lattice.stmt : complete_lattice stmt :=
+pi.complete_lattice
 
 def stmt.all {α} (s : α → stmt) : stmt :=
-λ L Γ D rip v, ∀ a, s a L Γ D rip v
+λ A D rip v, ∀ a, s a A D rip v
 
 def stmt.ex {α} (s : α → stmt) : stmt :=
-λ L Γ D rip v, ∃ a, s a L Γ D rip v
+λ A D rip v, ∃ a, s a A D rip v
 
 def stmt.with (p : Prop) (s : stmt) : stmt :=
 stmt.ex $ λ h : p, s
 
 def stmt.or (s₁ s₂ : stmt) : stmt :=
-λ L Γ D rip v, s₁ L Γ D rip v ∨ s₂ L Γ D rip v
+λ A D rip v, s₁ A D rip v ∨ s₂ A D rip v
 
 def stmt.stabilize (S : set place) (s : stmt) : stmt :=
-λ L Γ D, s L Γ (D ∪ S)
+λ A D, s A (D ∪ S)
 
 def expr (α : Type) := block → stmt
 
-instance has_le.expr {α} : has_le (expr α) :=
-⟨λ e₁ e₂, ∀ {{b}}, e₁ b ≤ e₂ b⟩
+instance complete_lattice.expr {α} : complete_lattice (expr α) :=
+pi.complete_lattice
 
-def expr.hoareIO {α} (L Γ) (P : sProp) (E : expr α)
+def expr.hoareIO {α} (A) (P : sProp) (E : expr α)
   (Q : block → list byte → list byte → mProp) : Prop :=
-∀ b, (E b).hoareIO L Γ P $
+∀ b, (E b).hoareIO A P $
   λ e i o, (Q b i o).with (e = exit_kind.straight)
 
-def expr.hoare {α} (L Γ) (P : sProp) (E : expr α) (Q : block → mProp) : Prop :=
-expr.hoareIO L Γ P E (λ ret i o, noIO (Q ret) i o)
+def expr.hoare {α} (A) (P : sProp) (E : expr α) (Q : block → mProp) : Prop :=
+expr.hoareIO A P E (λ ret i o, noIO (Q ret) i o)
 
 def expr.stabilize {α} (S : set place) (s : expr α) : expr α :=
 λ b, (s b).stabilize S
@@ -360,14 +377,14 @@ instance box.type (α) [type α] : type (box α) :=
     ⟨a, l, s', h₁.stable ss₁, h₂, type.read_stable h₃ ss₂, e⟩⟩
 
 def ret (α) (b : block) : expr α :=
-λ bl L Γ D a v, bl = b ∧ v = []
+λ bl A D a v, bl = b ∧ v = []
 
 def const (α) (l : list byte) : expr α := ret α (block.const l)
 
 def name (α : Type) := ℕ
 
 def var {α} (i : name α) : expr α :=
-λ bl L Γ D a v, bl ∈ Γ.get i ∧ v = []
+λ bl A D a v, bl ∈ A.read i ∧ v = []
 
 def hexpr {α} (P : sProp) (Q : block → mProp) : expr α :=
 λ ret, hstmt P (Q ret)
@@ -384,17 +401,17 @@ expr.ex $ λ h : p, s
 def const' {α} [type α] (a : α) : expr α :=
 hexpr ⊤ $ λ b, mProp.final mProp.id (type.read' a b)
 
-inductive stmt.seq (s₁ : stmt) (s₂ : stmt) : stmt
-| mk {L Γ D rip v₁ v₂} :
-  s₁ L Γ D rip v₁ →
-  s₂ L Γ D (rip + v₁.length) v₂ →
-  stmt.seq L Γ D rip (v₁ ++ v₂)
+inductive stmt.seq (s₁ s₂ : stmt) : stmt
+| mk {A D rip v₁ v₂} :
+  s₁ A D rip v₁ →
+  s₂ A D (rip + v₁.length) v₂ →
+  stmt.seq A D rip (v₁ ++ v₂)
 
 inductive expr.bindS {α} (e₁ : expr α) (s₂ : block → stmt) : stmt
-| mk {b L Γ D rip v₁ v₂} :
-  e₁ b L Γ D rip v₁ →
-  s₂ b L Γ D (rip + v₁.length) v₂ →
-  expr.bindS L Γ D rip (v₁ ++ v₂)
+| mk {b A D rip v₁ v₂} :
+  e₁ b A D rip v₁ →
+  s₂ b A D (rip + v₁.length) v₂ →
+  expr.bindS A D rip (v₁ ++ v₂)
 
 def expr.bind {α β} (e₁ : expr α) (e₂ : block → expr β) : expr β :=
 λ b₂, expr.bindS e₁ $ λ b₁, e₂ b₁ b₂
@@ -408,12 +425,12 @@ expr.bindS e₁ $ λ dst, expr.bindS e₂ $ λ src, block.mov dst src
 
 inductive label | fail | label (n : ℕ)
 
-inductive label.loc (L : labels_ctx) : label → qword → Prop
-| fail : label.loc label.fail L.1
-| label (n h) : label.loc (label.label n) (L.2.nth_le n h)
+inductive label.loc (A : asm_ctx) : label → qword → Prop
+| fail : label.loc label.fail A.exit
+| label (n h) : label.loc (label.label n) (A.L.nth_le n h)
 
 def stmt.jump_cc (p : flags → bool) (l : label) : stmt :=
-λ L Γ D rip v, ∀ tgt, l.loc L tgt →
+λ A D rip v, ∀ tgt, l.loc A tgt →
 mHoare (sProp.sn place.rip rip ⊓ sProp.mem_block (perm.R + perm.X) rip v)
   (λ k k', stable_at D k k' ∧
     mProp.write place.rip (cond (p k.flags) tgt (rip + v.length)) k k')
@@ -422,8 +439,8 @@ def stmt.jump : label → stmt := stmt.jump_cc (λ _, tt)
 
 def boolexpr := (flags → bool) → stmt
 
-def boolexpr.hoare (L Γ) (P : sProp) (E : boolexpr) (Q : bool → mProp) : Prop :=
-∃ p, stmt.hoare L Γ P (E p)
+def boolexpr.hoare (A) (P : sProp) (E : boolexpr) (Q : bool → mProp) : Prop :=
+∃ p, stmt.hoare A P (E p)
   (λ e k k', e = exit_kind.straight ∧ Q (p k'.flags) k k')
 
 def boolexpr.not (c : boolexpr) : boolexpr :=
@@ -432,21 +449,21 @@ def boolexpr.not (c : boolexpr) : boolexpr :=
 def boolexpr.jump_if (c : boolexpr) (l : label) : stmt :=
 stmt.ex $ λ p, (c p).seq $ stmt.jump_cc p l
 
-def stmt.nop : stmt := λ L Γ D rip v, v = []
+def stmt.nop : stmt := λ A D rip v, v = []
 
 def if_stmt (c : boolexpr) (s₁ s₂ : stmt) : stmt :=
-stmt.ex $ λ p, stmt.seq (c p) $ λ L Γ D rip v,
+stmt.ex $ λ p, stmt.seq (c p) $ λ A D rip v,
 ∃ v₁ v₂ v₃, v = v₁ ++ v₂ ++ v₃ ∧
 let q₁ := rip + v₁.length, q₂ := q₁ + v₂.length in
-stmt.jump_cc (bnot ∘ p) (label.label 0) (L.cons q₁) Γ D rip v₁ ∧
-s₁.seq (stmt.jump (label.label 0)) (L.cons q₂) Γ D q₁ v₂ ∧
-s₂.seq (stmt.jump (label.label 0)) (L.cons q₂) Γ D q₂ v₃
+stmt.jump_cc (bnot ∘ p) (label.label 0) (A.push_label q₁) D rip v₁ ∧
+s₁.seq (stmt.jump (label.label 0)) (A.push_label q₂) D q₁ v₂ ∧
+s₂.seq (stmt.jump (label.label 0)) (A.push_label q₂) D q₂ v₃
 
 def loop (s : stmt) : stmt :=
-λ L Γ D rip, s (L.cons rip) Γ D rip
+λ A D rip, s (A.push_label rip) D rip
 
 def block_stmt (s : stmt) : stmt :=
-λ L Γ D rip v, s (L.cons (rip + v.length)) Γ D rip v
+λ A D rip v, s (A.push_label (rip + v.length)) D rip v
 
 def while (c : boolexpr) (s : stmt) : stmt :=
 block_stmt $ loop $
@@ -455,7 +472,7 @@ block_stmt $ loop $
   stmt.jump (label.label 0)
 
 def decl_block {α} (b : block) (s : name α → stmt) : stmt :=
-λ L Γ D rip v, ∃ i, s i L (Γ.insert i b) D rip v
+λ A D rip v, ∃ i, s i (A.push_local i b) D rip v
 
 def decl {α} (sz : qword) (s : name α → stmt) : stmt :=
 stmt.ex $ λ b, stmt.with (block.size b = sz) $ decl_block b s
@@ -465,7 +482,7 @@ e.bindS $ λ b, decl_block b s
 
 def binop_expr {α β γ} [type α] [type β] [type γ]
   (f : α → β → γ) (e₁ : expr α) (e₂ : expr β) : expr γ :=
-e₁.bind $ λ b₁, e₂.bind $ λ b₂ b, stmt.ex $ λ x, stmt.ex $ λ y,
+e₁.bind $ λ b₁, e₂.bind $ λ b₂ b, stmt.all $ λ x, stmt.all $ λ y,
 hstmt (type.read' x b₁ ⊓ type.read' y b₂) (type.write (f x y) b)
 
 def asn_binop {α β} [type α] [type β] (f : α → β → α) (e₁ : expr α) (e₂ : expr β) : stmt :=
@@ -501,14 +518,69 @@ for (const' (0 : qword)) (λ i, ltq (const' 0) max) (λ i, incr (var i)) body
 -- Program logic
 ----------------------------------------
 
-theorem hoare_p.mono {P P' : kcfg → Prop}
-  (H : ∀ {{k}}, P k → P' k) {k} : hoare_p P k → hoare_p P' k :=
+theorem mProp.comp_imp {P Q} : mProp.comp P (mProp.imp P Q) ≤ Q :=
+λ k₁ k₃ ⟨k₂, h₁, h₂⟩, h₂ _ h₁
+
+theorem mProp.comp_ex_imp {α P Q} :
+  mProp.comp (@mProp.ex α P) (mProp.all $ λ a, mProp.imp (P a) Q) ≤ Q :=
+λ k₁ k₃ ⟨k₂, ⟨a, h₁⟩, h₂⟩, h₂ a _ h₁
+
+theorem mProp.ex_apply {α Q P} :
+  (@mProp.ex α Q).apply P = sProp.ex (λ a, (Q a).apply P) :=
+funext $ λ k, propext
+⟨λ ⟨k', h₁, a, h₂⟩, ⟨a, k', h₁, h₂⟩,
+ λ ⟨a, k', h₁, h₂⟩, ⟨k', h₁, a, h₂⟩⟩
+
+theorem mProp.ex_comp {α Q Q'} :
+  (@mProp.ex α Q).comp Q' = mProp.ex (λ a, (Q a).comp Q') :=
+funext $ λ k, funext $ λ k', propext
+⟨λ ⟨k'', ⟨a, h₁⟩, h₂⟩, ⟨a, k'', h₁, h₂⟩,
+ λ ⟨a, k'', h₁, h₂⟩, ⟨k'', ⟨a, h₁⟩, h₂⟩⟩
+
+theorem mem.read'_left {m p a v₁ v₂} (ss : v₁ <+: v₂) :
+  mem.read' m p a v₂ → mem.read' m p a v₁ :=
+begin
+  intro h, induction h generalizing v₁,
+  { cases list.eq_nil_of_prefix_nil ss, constructor },
+  { cases v₁, constructor,
+    rcases ss with ⟨_, ⟨⟩⟩,
+    exact mem.read'.cons h_a (h_ih ⟨_, rfl⟩) }
+end
+
+theorem mem.read'_right {m p a v₁ v₂} :
+  mem.read' m p a (v₁ ++ v₂) → mem.read' m p (a + v₁.length) v₂ :=
+begin
+  generalize e : v₁ ++ v₂ = v,
+  intro h, induction h generalizing v₁ v₂,
+  { cases list.eq_nil_of_suffix_nil ⟨_, e⟩, constructor },
+  { cases v₁; cases e,
+    { simp, exact mem.read'.cons h_a h_a_1 },
+    { simp [-add_comm], rw [← add_assoc, add_right_comm],
+      exact h_ih rfl } }
+end
+
+theorem hoare_p.bind {P P' : kcfg → Prop}
+  (H : ∀ {{k}}, P k → hoare_p P' k) {k} : hoare_p P k → hoare_p P' k :=
 begin
   intro h, induction h,
-  exact hoare_p.zero (H h_a),
+  exact H h_a,
   exact hoare_p.step h_a (λ k', h_ih _),
-  exact hoare_p.exit _ _ h_a (λ e, H (h_a_1 e)),
+  by_cases h_ret = 0,
+  { cases H (h_a_1 h),
+    { exact hoare_p.zero a },
+    { rcases a with ⟨_, ⟨_, _, _, _, h'⟩ | ⟨_, _, _, _, _, _, _, _, h'⟩⟩,
+      { cases config.step_no_exit h' h_a },
+      { rcases h_a with ⟨k₁, h₁, ⟨e⟩⟩,
+        cases config.isIO.determ h' h₁,
+        generalize_hyp : a_h_k₁.regs RAX = r at e a_h_a,
+        induction a_h_a; cases bitvec.reify_eq₂ e } },
+    { exact hoare_p.exit _ _ a a_1 } },
+  { exact hoare_p.exit _ _ h_a h.elim },
 end
+
+theorem hoare_p.mono {P P' : kcfg → Prop}
+  (H : ∀ {{k}}, P k → P' k) {k} : hoare_p P k → hoare_p P' k :=
+hoare_p.bind (λ k h, hoare_p.zero (H h))
 
 theorem hoare.zero {P : kcfg → Prop} {Q : kcfg → kcfg → Prop}
   (H : ∀ {{k}}, P k → Q k k) : hoare P Q :=
@@ -525,40 +597,73 @@ theorem hoare.mono_l {P P' : kcfg → Prop} {Q : kcfg → kcfg → Prop}
 λ H' k h, H' (H h)
 
 theorem hoare.mono_r {P : kcfg → Prop} {Q Q' : kcfg → kcfg → Prop}
-  (H : ∀ {{k k'}}, Q k k' → Q' k k') : hoare P Q → hoare P Q' :=
-λ H' k h, hoare_p.mono (@H _) (H' h)
+  (H : ∀ {{k k'}}, P k → Q k k' → Q' k k') : hoare P Q → hoare P Q' :=
+λ H' k h, hoare_p.mono (λ k' h', H h (by exact h')) (H' h)
+
+theorem hoare.comp {P : kcfg → Prop} {Q Q' : kcfg → kcfg → Prop}
+  (H₁ : hoare P Q)
+  (H₂ : hoare (λ k', ∃ k, Q k k' ∧ P k) Q') :
+  hoare P (rel.comp Q Q') :=
+λ k p, begin
+  refine (hoare.mono_r _ H₁ p).bind _,
+  exact (λ k k', Q k k' ∧ P k),
+  rintro k' ⟨h₁, h₂⟩,
+  refine (H₂ ⟨_, h₁, h₂⟩).mono (λ k₂ h, ⟨_, h₁, h⟩),
+  exact λ k k' h₁ h₂, ⟨h₂, h₁⟩
+end
 
 theorem mHoareIO.zero {P : sProp} {Q : list byte → list byte → mProp}
   (H : ∀ {{k}}, P k → Q [] [] k k) : mHoareIO P Q :=
-λ i o, hoare.zero $ by rintro k ⟨h, rfl, rfl⟩; exact
-  ⟨[], [], rfl, (list.append_nil _).symm, H h⟩
+hoare.zero $ λ k h, ⟨[], [], rfl, (list.append_nil _).symm, H h⟩
 
 theorem mHoareIO.mono_l {P P' : sProp} {Q : list byte → list byte → mProp}
   (H : P ≤ P') : mHoareIO P' Q → mHoareIO P Q :=
-λ h i o, hoare.mono_l (by exact λ k ⟨h₁, h₂⟩, ⟨H h₁, h₂⟩) (@h i o)
+λ h, hoare.mono_l (λ k h, H _ h) h
 
 theorem mHoareIO.mono_r {P : sProp} {Q Q' : list byte → list byte → mProp}
   (H : ∀ {{i o}}, Q i o ≤ Q' i o) : mHoareIO P Q → mHoareIO P Q' :=
-λ h i o, hoare.mono_r (by exact λ k k' ⟨i', o', h₁, h₂, h₃⟩,
-  ⟨i', o', h₁, h₂, H h₃⟩) (@h i o)
+λ h, hoare.mono_r (by exact λ k k' _ ⟨i', o', h₁, h₂, h₃⟩,
+  ⟨i', o', h₁, h₂, H _ _ h₃⟩) h
 
 theorem mHoareIO.step {P P' : sProp} {Q Q' : list byte → list byte → mProp}
   (H₁ : ∀ ⦃k i o⦄, P k → ∃ k', kcfg.step ⟨i, o, k⟩ k')
-  (H₂ : ∀ {{k₁ i₁ o₁ k₂ i₂ o₂}}, P k₁ →
-    kcfg.step ⟨i₁, o₁, k₁⟩ ⟨i₂, o₂, k₂⟩ → P' k₂ ∧ i₂ = i₁ ∧ o₂ = o₁ ∧
-      ∀ {{k₃}}, Q' [] [] k₂ k₃ → Q [] [] k₁ k₃)
+  (H₂ : ∀ {{k₁ k₂ i o i₁ o₁}}, P k₁ →
+    kcfg.step ⟨i₁ ++ i, o, k₁⟩ ⟨i, o ++ o₁, k₂⟩ → P' k₂ ∧
+      ∀ {{i₂ o₂ k₃}}, Q' i₂ o₂ k₂ k₃ → Q (i₁ ++ i₂) (o₁ ++ o₂) k₁ k₃)
   (H₃ : mHoareIO P' Q') : mHoareIO P Q :=
-λ i o, begin
-  refine hoare.step (λ ⟨i', o', k⟩ h, H₁ h.1) _ (@H₃ i o),
-  rintro ⟨i₁, o₁, k₁⟩ ⟨h, rfl, rfl⟩ ⟨i₂, o₂, k₂⟩ h',
-  rcases @H₂ k₁ i₁ o₁ k₂ i₂ o₂ h h' with ⟨h₁, rfl, rfl, h₄⟩,
-  refine ⟨⟨h₁, rfl, rfl⟩, _⟩,
+begin
+  refine hoare.step (λ ⟨i', o', k⟩ h, H₁ h) _ H₃,
+  rintro ⟨i₁, o₁, k₁⟩ h ⟨i₂, o₂, k₂⟩ h',
+  rcases kcfg.step.io_part h' with ⟨⟨i, rfl⟩, ⟨o, rfl⟩⟩,
+  rcases H₂ h h' with ⟨h₁, h₄⟩,
+  refine ⟨h₁, _⟩,
   rintro k₃ ⟨i', o', e₁, e₂, h₅⟩,
-  refine ⟨i', o', e₁, e₂, _⟩,
-  cases ((list.append_right_inj _).1 e₁ : [] = i'),
-  cases ((list.append_left_inj _).1 ((list.append_nil _).trans e₂) : [] = o'),
-  exact h₄ h₅
+  exact ⟨_, _,
+    (congr_arg ((++) i) e₁).trans (list.append_assoc _ _ _).symm,
+    e₂.trans (list.append_assoc _ _ _),
+    h₄ h₅⟩
 end
+
+theorem mHoareIO.comp {P : sProp} {Q Q' : list byte → list byte → mProp}
+  (H₁ : mHoareIO P Q)
+  (H₂ : mHoareIO (sProp.ex $ λ i, sProp.ex $ λ o, (Q i o).apply P) Q') :
+  mHoareIO P (λ i o,
+    mProp.ex $ λ i₁, mProp.ex $ λ i₂,
+    mProp.ex $ λ o₁, mProp.ex $ λ o₂,
+    ((Q i₁ o₁).comp (Q' i₂ o₂)).with (i = i₁ ++ i₂ ∧ o = o₁ ++ o₂)) :=
+λ k p, begin
+  refine (H₁ p).bind _,
+  rintro k₁ ⟨i₁, o₁, e₁, e₂, h₁⟩,
+  refine (H₂ ⟨_, _, _, p, h₁⟩).mono _,
+  rintro k₂ ⟨i₂, o₂, e₃, e₄, h₂⟩,
+  refine ⟨_, _, _, _, _, _, _, _, ⟨_, h₁, h₂⟩, rfl, rfl⟩,
+  rw [e₁, list.append_assoc, e₃],
+  rw [e₄, ← list.append_assoc, e₂],
+end
+
+theorem mHoareIO.ex_l {α} {P : α → sProp} {Q} :
+  mHoareIO (sProp.ex P) Q ↔ ∀ a, mHoareIO (P a) Q :=
+⟨λ H a k h, H ⟨a, h⟩, λ H k ⟨a, h⟩, H a h⟩
 
 theorem mHoare.zero {P : sProp} {Q : mProp}
   (H : ∀ {{k}}, P k → Q k k) : mHoare P Q :=
@@ -570,7 +675,7 @@ mHoareIO.mono_l H
 
 theorem mHoare.mono_r {P : sProp} {Q Q' : mProp}
   (H : Q ≤ Q') : mHoare P Q → mHoare P Q' :=
-mHoareIO.mono_r $ λ k k' i o ⟨h₁, h₂, h₃⟩, ⟨H h₁, h₂, h₃⟩
+mHoareIO.mono_r $ λ k k' i o ⟨h₁, h₂, h₃⟩, ⟨H _ _ h₁, h₂, h₃⟩
 
 theorem mHoare.step {P P' : sProp} {Q Q' : mProp}
   (H₁ : ∀ ⦃k⦄, P k → ∃ k', config.step k k')
@@ -579,94 +684,211 @@ theorem mHoare.step {P P' : sProp} {Q Q' : mProp}
   mHoare P' Q' → mHoare P Q :=
 mHoareIO.step
   (λ k i o h, let ⟨k', h'⟩ := H₁ h in ⟨⟨i, o, k'⟩, kcfg.step.noio h'⟩)
-  (λ k₁ i₁ o₁ k₂ i₂ o₂ h h', begin
+  (λ k₁ k₂ i o i₁ o₁ h h', begin
+    generalize_hyp ei : i₁ ++ i = i' at h',
+    generalize_hyp eo : o ++ o₁ = o' at h',
     cases h',
-    { exact ⟨(H₂ h h'_a).1, rfl, rfl,
-        λ k₃ h'', ⟨(H₂ h h'_a).2 h''.1, rfl, rfl⟩⟩ },
+    { cases (@list.append_right_inj _ _ [] i).1 ei,
+      cases (@list.append_left_inj _ _ [] o).1 (by simpa using eo),
+      exact ⟨(H₂ h h'_a).1,
+        λ i₂ o₂ k₃ h'', ⟨(H₂ h h'_a).2 h''.1, h''.2⟩⟩ },
     { cases H₁ h with k₂ h',
       cases config.step_noIO h' h'_a }
   end)
 
-theorem stmt.hoareIO.mono_s {L Γ P Q s₁ s₂}
-  (h : s₂ ≤ s₁) : stmt.hoareIO L Γ P s₁ Q → stmt.hoareIO L Γ P s₂ Q :=
-λ H D rip l h', H _ _ _ (h h')
+theorem mHoare.comp {P : sProp} {Q Q' : mProp}
+  (H₁ : mHoare P Q)
+  (H₂ : mHoare (Q.apply P) Q') :
+  mHoare P (Q.comp Q') :=
+(H₁.comp (H₂.mono_l
+  (λ k₂ ⟨_, _, k₁, h₁, h₂, rfl, rfl⟩, ⟨_, h₁, h₂⟩))).mono_r $
+by rintro _ _ k₁ k₃ ⟨i₁, o₁, i₂, o₂,
+    ⟨k₂, ⟨h₁, rfl, rfl⟩, ⟨h₂, rfl, rfl⟩⟩, rfl, rfl⟩;
+  exact ⟨⟨_, h₁, h₂⟩, rfl, rfl⟩
 
-theorem stmt.hoareIO.mono_l {L Γ P₁ P₂ s Q}
-  (h : P₂ ≤ P₁) : stmt.hoareIO L Γ P₁ s Q → stmt.hoareIO L Γ P₂ s Q :=
+theorem mHoare.ex_l {α} {P : α → sProp} {Q} :
+  mHoare (sProp.ex P) Q ↔ ∀ a, mHoare (P a) Q :=
+⟨λ H a k h, H ⟨a, h⟩, λ H k ⟨a, h⟩, H a h⟩
+
+theorem stmt.hoareIO.mono_s {A P Q s₁ s₂}
+  (h : s₂ ≤ s₁) : stmt.hoareIO A P s₁ Q → stmt.hoareIO A P s₂ Q :=
+λ H D rip l h', H _ _ _ (h _ _ _ _ h')
+
+theorem stmt.hoareIO.mono_l {A P₁ P₂ s Q}
+  (h : P₂ ≤ P₁) : stmt.hoareIO A P₁ s Q → stmt.hoareIO A P₂ s Q :=
 λ H D rip l h', (H _ _ _ h').mono_l
-  (λ k ⟨⟨h₁, h₂⟩, h₃⟩, ⟨⟨h h₁, h₂⟩, h₃⟩)
+  (λ k ⟨⟨h₁, h₂⟩, h₃⟩, ⟨⟨h _ h₁, h₂⟩, h₃⟩)
 
-theorem stmt.hoareIO.mono_r {L Γ P s}
+theorem stmt.hoareIO.mono_r {A P s}
   {Q₁ Q₂ : exit_kind → list byte → list byte → mProp}
   (h : ∀ {{e i o}}, Q₁ e i o ≤ Q₂ e i o) :
-  stmt.hoareIO L Γ P s Q₁ → stmt.hoareIO L Γ P s Q₂ :=
+  stmt.hoareIO A P s Q₁ → stmt.hoareIO A P s Q₂ :=
 λ H D rip l h', (H _ _ _ h').mono_r
-  (λ i o k k', and.imp_right $ or.imp_right $
-    Exists.imp $ λ e, and.imp_left $ λ h₁, h h₁)
+  (λ i o k k', and.imp_right $
+    Exists.imp $ λ e, and.imp_left $ λ h₁, h _ _ h₁)
 
-theorem expr.hoare.zero {α} {L Γ P} {e : expr α} {p : block → Prop}
-  (H : ∀ {{b D rip l}}, e b L Γ D rip l → p b ∧ l = []) :
-  e.hoare L Γ P (λ b, mlift (p b)) :=
-λ b D rip l h', begin
-  rcases H h' with ⟨h, rfl⟩, apply mHoareIO.zero,
-  rintro k ⟨⟨h₁, h₂⟩, h₃⟩,
-  refine ⟨stable_at.zero, or.inr ⟨_, ⟨⟨h, rfl, rfl⟩, rfl⟩, _⟩⟩,
-  change place.write _ _ (rip + 0) _,
-  rw bitvec.add_zero,
-  convert place.write.rip k,
-  cases k, cases h₂, refl
+theorem stmt.hoareIO.ex_l {α A s} {P : α → sProp} {Q} :
+  stmt.hoareIO A (sProp.ex P) s Q ↔ ∀ a, stmt.hoareIO A (P a) s Q :=
+⟨λ H a, H.mono_l $ λ k h, ⟨a, h⟩,
+ λ H S rip k h k ⟨⟨⟨a, h₁⟩, h₂⟩, h₃⟩,
+  H a _ _ _ h ⟨⟨h₁, h₂⟩, h₃⟩⟩
+
+theorem stmt.hoare_iff {A P s Q} :
+  stmt.hoare A P s Q ↔
+  ∀ {{D rip l}}, s A D rip l →
+    mHoare
+      (P ⊓ sProp.sn place.rip rip ⊓
+        sProp.mem_block (perm.R + perm.X) rip l)
+      (mProp.ex (λ e, stable_at D ⊓
+        (Q e).final (e.result A (rip + l.length)))) :=
+forall_congr $ λ D, forall_congr $ λ rip, forall_congr $ λ l,
+forall_congr $ λ h, iff_of_eq begin
+  congr, funext i o k k', exact propext
+    ⟨λ ⟨h₁, e, ⟨h₂, ei, eo⟩, h₃⟩, ⟨⟨e, h₁, h₂, h₃⟩, ei, eo⟩,
+     λ ⟨⟨e, h₁, h₂, h₃⟩, ei, eo⟩, ⟨h₁, e, ⟨h₂, ei, eo⟩, h₃⟩⟩,
 end
 
-theorem expr.hoareIO.mono_e {α L Γ P Q} {e₁ e₂ : expr α}
-  (h : e₂ ≤ e₁) : expr.hoareIO L Γ P e₁ Q → expr.hoareIO L Γ P e₂ Q :=
+theorem stmt.hoare.mono_s {A P Q s₁ s₂}
+  (h : s₂ ≤ s₁) : stmt.hoare A P s₁ Q → stmt.hoare A P s₂ Q :=
+λ H D rip l h', H _ _ _ (h _ _ _ _ h')
+
+theorem stmt.hoare.mono_l {A P₁ P₂ s Q}
+  (h : P₂ ≤ P₁) : stmt.hoare A P₁ s Q → stmt.hoare A P₂ s Q :=
+λ H D rip l h', (H _ _ _ h').mono_l
+  (λ k ⟨⟨h₁, h₂⟩, h₃⟩, ⟨⟨h _ h₁, h₂⟩, h₃⟩)
+
+theorem stmt.hoare.mono_r {A P s} {Q₁ Q₂ : exit_kind → mProp}
+  (h : ∀ {{e}}, Q₁ e ≤ Q₂ e) :
+  stmt.hoare A P s Q₁ → stmt.hoare A P s Q₂ :=
+stmt.hoareIO.mono_r $ λ e i o k k' ⟨h₁, h₂⟩, ⟨h _ _ h₁, h₂⟩
+
+theorem stmt.hoare.zero {A P} {s : stmt} {p : Prop}
+  (H : ∀ {{D rip l}}, s A D rip l → p ∧ l = []) :
+  s.hoare A P (λ e, (mlift p).with (e = exit_kind.straight)) :=
+stmt.hoare_iff.2 $ λ D rip l h', begin
+  rcases H h' with ⟨h, rfl⟩, apply mHoare.zero,
+  rintro k ⟨⟨h₁, h₂⟩, h₃⟩,
+  refine ⟨_, stable_at.refl, ⟨h, rfl⟩, _⟩,
+  simpa using h₂
+end
+
+theorem stmt.hoare.ex_l {α A s} {P : α → sProp} {Q} :
+  stmt.hoare A (sProp.ex P) s Q ↔ ∀ a, stmt.hoare A (P a) s Q :=
+⟨λ H a, H.mono_l $ λ k h, ⟨a, h⟩,
+ λ H S rip k h k ⟨⟨⟨a, h₁⟩, h₂⟩, h₃⟩,
+  H a _ _ _ h ⟨⟨h₁, h₂⟩, h₃⟩⟩
+
+theorem expr.hoare_iff {α A P E Q} :
+  @expr.hoare α A P E Q ↔
+  ∀ {{b}}, (E b).hoare A P $
+    λ e, (Q b).with (e = exit_kind.straight) :=
+forall_congr $ λ b, iff_of_eq begin
+  congr, funext e i o k k', exact propext
+    ⟨λ ⟨⟨h, ei, eo⟩, ee⟩, ⟨⟨h, ee⟩, ei, eo⟩,
+     λ ⟨⟨h, ee⟩, ei, eo⟩,  ⟨⟨h, ei, eo⟩, ee⟩⟩
+end
+
+theorem expr.hoare.zero {α A P} {e : expr α} {p : block → Prop}
+  (H : ∀ {{b D rip l}}, e b A D rip l → p b ∧ l = []) :
+  e.hoare A P (λ b, mlift (p b)) :=
+expr.hoare_iff.2 $ λ b, stmt.hoare.zero (@H b)
+
+theorem expr.hoareIO.mono_e {α A P Q} {e₁ e₂ : expr α}
+  (h : e₂ ≤ e₁) : expr.hoareIO A P e₁ Q → expr.hoareIO A P e₂ Q :=
 λ H b, (H b).mono_s (@h b)
 
-theorem expr.hoareIO.mono_l {α L Γ P₁ P₂ s Q}
-  (h : P₂ ≤ P₁) : @expr.hoareIO α L Γ P₁ s Q → expr.hoareIO L Γ P₂ s Q :=
+theorem expr.hoareIO.mono_l {α A P₁ P₂ s Q}
+  (h : P₂ ≤ P₁) : @expr.hoareIO α A P₁ s Q → expr.hoareIO A P₂ s Q :=
 λ H b, (H b).mono_l h
 
-theorem expr.hoareIO.mono_r {α L Γ P s}
+theorem expr.hoareIO.mono_r {α A P s}
   {Q₁ Q₂ : block → list byte → list byte → mProp}
   (h : ∀ {{b i o}}, Q₁ b i o ≤ Q₂ b i o) :
-  @expr.hoareIO α L Γ P s Q₁ → expr.hoareIO L Γ P s Q₂ :=
-λ H b, (H b).mono_r $ λ e i o k k', and.imp_left $ λ h₁, h h₁
+  @expr.hoareIO α A P s Q₁ → expr.hoareIO A P s Q₂ :=
+λ H b, (H b).mono_r $ λ e i o, inf_le_inf (@h _ _ _) (le_refl _)
 
-theorem var.hoare {α} (i : name α) {L Γ} (P : sProp) :
-  (var i).hoare L Γ P (λ b, mlift (b ∈ Γ.get i)) :=
+theorem expr.hoareIO.ex_l {α β A} {e : expr β} {P : α → sProp} {Q} :
+  expr.hoareIO A (sProp.ex P) e Q ↔ ∀ a, expr.hoareIO A (P a) e Q :=
+iff.trans (forall_congr $ λ b, stmt.hoareIO.ex_l) forall_swap
+
+theorem expr.to_hoare {α A P} {e : expr α} {Q : block → mProp}
+  (H : ∀ b, stmt.hoare A P (e b) (λ e, (Q b).with (e = exit_kind.straight))) :
+  expr.hoare A P e Q :=
+begin
+  refine λ b, stmt.hoareIO.mono_r _ (H b),
+  rintro e _ _ k k' ⟨⟨h, e'⟩, rfl, rfl⟩, exact ⟨⟨h, rfl, rfl⟩, e'⟩
+end
+
+theorem expr.hoare.ex_l {α β A} {e : expr β} {P : α → sProp} {Q} :
+  expr.hoare A (sProp.ex P) e Q ↔ ∀ a, expr.hoare A (P a) e Q :=
+expr.hoareIO.ex_l
+
+theorem var.hoare {α} (i : name α) {A} (P : sProp) :
+  (var i).hoare A P (λ b, mlift (b ∈ A.read i)) :=
 expr.hoare.zero $ λ _ _ _ _, id
 
-theorem ret.hoare {α b L Γ} (P : sProp) :
-  (ret α b).hoare L Γ P (λ b', mlift (b' = b)) :=
+theorem ret.hoare {α b A} (P : sProp) :
+  (ret α b).hoare A P (λ b', mlift (b' = b)) :=
 expr.hoare.zero $ λ _ _ _ _, id
 
-theorem hstmt.hoare {L Γ} (P : sProp) (Q : mProp) :
-  (hstmt P Q).hoare L Γ P (λ e, Q.with (e = exit_kind.straight)) :=
-λ D rip l h',
-(mHoareIO.mono_l
+theorem hstmt.hoare {A} (P : sProp) (Q : mProp) :
+  (hstmt P Q).hoare A P (λ e, Q.with (e = exit_kind.straight)) :=
+stmt.hoare_iff.2 $ λ D rip l h',
+(mHoare.mono_l
   (by exact λ _, and.imp_left and.right) h').mono_r $
-by rintro i o k k' ⟨⟨⟨h₁, h₂⟩, h₃⟩, rfl, rfl⟩; exact
-  ⟨h₂, or.inr ⟨_, ⟨⟨h₁, rfl⟩, rfl, rfl⟩, h₃⟩⟩
+by rintro k k' ⟨⟨h₁, h₂⟩, h₃⟩; exact ⟨_, h₂, ⟨h₁, rfl⟩, h₃⟩
 
-theorem hexpr.hoare {α L Γ} (P : sProp) (Q : block → mProp) :
-  (@hexpr α P Q).hoare L Γ P Q :=
-λ b D rip l h',
-(mHoareIO.mono_l
-  (by exact λ _, and.imp_left and.right) h').mono_r $
-by rintro i o k k' ⟨⟨⟨h₁, h₂⟩, h₃⟩, rfl, rfl⟩; exact
-  ⟨h₂, or.inr ⟨_, ⟨⟨h₁, rfl, rfl⟩, rfl⟩, h₃⟩⟩
+theorem hexpr.hoare {α A} (P : sProp) (Q : block → mProp) :
+  (@hexpr α P Q).hoare A P Q :=
+expr.to_hoare $ λ b, hstmt.hoare _ _
+
+def comp_exit (Q₁ Q₂ : exit_kind → mProp) (e : exit_kind) : mProp :=
+mProp.ex $ λ e₁, exit_kind.cases_on e₁ ((Q₁ e₁).comp (Q₂ e)) $ λ _, (Q₁ e₁).with (e₁ = e)
+
+theorem stmt.seq.hoare {A s₁ s₂}
+  {P₁ P₂ : sProp} {Q₁ Q₂ : exit_kind → mProp}
+  (H₁ : stmt.hoare A P₁ s₁ Q₁)
+  (H₂ : stmt.hoare A P₂ s₂ Q₂)
+  (H : (Q₁ exit_kind.straight).apply P₁ ≤ P₂) :
+  (stmt.seq s₁ s₂).hoare A P₁ (comp_exit Q₁ Q₂) :=
+stmt.hoare_iff.2 begin
+  rintro D rip l ⟨_, _, _, v₁, v₂, h₁, h₂⟩,
+  change v₁.append v₂ with v₁ ++ v₂ at a ⊢,
+  have := stmt.hoare_iff.1 H₁ h₁,
+  refine (((stmt.hoare_iff.1 H₁ h₁).mono_l _).comp _).mono_r mProp.comp_ex_imp,
+  { refine inf_le_inf (le_refl _) _,
+    exact λ k, mem.read'_left ⟨_, rfl⟩ },
+  rw [mProp.ex_apply, mHoare.ex_l], rintro (_|⟨n⟩),
+  { refine ((stmt.hoare_iff.1 H₂ h₂).mono_l _).mono_r _,
+    rintro k₂ k₃ ⟨e₂, s₂, q₂, r₂⟩ e₁ k₁ ⟨s₁, q₁, r₁⟩,
+    rw [list.length_append, ← bitvec.add_nat_assoc],
+    refine ⟨e₂, s₁.trans s₂, _⟩,
+    exact ⟨⟨exit_kind.straight, _, q₁, q₂⟩, r₂⟩ },
+  { exact ⟨⟨exit_kind.label n, q₁, _⟩, r₂⟩ },
+
+  have:= (((stmt.hoare_iff.1 H₁ h₁).mono_l _).comp
+          ((stmt.hoare_iff.1 H₂ h₂).mono_l _)).mono_r _,
+  { rintro k₁ k₃ ⟨k₂, ⟨s₁, e₁, q₁, r₁⟩, ⟨s₂, e₂, q₂, r₂⟩⟩,
+    cases e₁,
+    { refine ⟨s₁.trans s₂, e₂, ⟨exit_kind.straight, _, q₁, q₂⟩, _⟩,
+      rwa [list.length_append, ← bitvec.add_nat_assoc] },
+    { refine ⟨s₁.trans s₂, _, ⟨exit_kind.label e₁, _, rfl⟩, _⟩,
+
+    } },
+end
 
 ----------------------------------------
 -- Assembly
 ----------------------------------------
 
-theorem var.asm {α} {i : name α} {L Γ D rip bl}
-  (h : bl ∈ locals_ctx.get Γ i) : var i bl L Γ D rip [] :=
+theorem var.asm {α} {i : name α} {A D rip bl}
+  (h : bl ∈ locals_ctx.get Γ i) : var i bl A D rip [] :=
 ⟨h, rfl⟩
 
-theorem ret.asm {α L Γ D rip bl} : ret α bl bl L Γ D rip [] :=
+theorem ret.asm {α A D rip bl} : ret α bl bl A D rip [] :=
 ⟨rfl, rfl⟩
 
-def stmt.asm (s : stmt) (D : set place) := Π L Γ rip, ∃ v, s L Γ D rip v
+def stmt.asm (s : stmt) (D : set place) := Π A rip, ∃ v, s A D rip v
 
 
 end x86
